Refactored the modular reification wrappers.

theories/Reify/ReifyView.v
@@ -46,29 +46,27 @@ Section ReifyFunc.
 
   Polymorphic Let Ext (x : SymEnv.func) := @ExprCore.Inj typ func (f_insert x).
 
-  Polymorphic Definition reify_func (rf : list (Command (expr typ func))) : Command (expr typ func) :=
+  Polymorphic Definition reify_func_aux (rf_pre rf_post : list (Command (expr typ func))) : Command (expr typ func) :=
     @Patterns.CFix (expr typ func)
       (@Patterns.CFirst_ _
-        (rf ++
+        (rf_pre ++
          ((Patterns.CVar (@ExprCore.Var typ func)) ::
           (Patterns.CApp (Patterns.CRec 0) (Patterns.CRec 0) (@ExprCore.App typ func)) ::
 	  (Patterns.CAbs (CCall (reify_scheme typ)) (CRec 0) (@ExprCore.Abs typ func)) ::
-	  (Patterns.CMap Ext (Patterns.CTypedTable (reify_scheme typ) term_table))::nil))).
+	  rf_post))).
+
+  Polymorphic Definition reify_func (rf : list (Command (expr typ func))) : Command (expr typ func) :=
+    reify_func_aux rf (Patterns.CMap Ext (Patterns.CTypedTable (reify_scheme typ) term_table)::nil).
+
+  Polymorphic Definition reify_func_no_table (rf : list (Command (expr typ func))) : Command (expr typ func) :=
+    reify_func_aux rf nil.
 
   Polymorphic Instance Reify_func (rf : list (Command (expr typ func))) : Reify (expr typ func) := {
     reify_scheme := reify_func rf
   }.
 
-  Polymorphic Definition reify_func' (rf : list (Command (expr typ func))) : Command (expr typ func) :=
-    @Patterns.CFix (expr typ func)
-      (@Patterns.CFirst_ _
-        (rf ++
-         ((Patterns.CVar (@ExprCore.Var typ func)) ::
-          (Patterns.CApp (Patterns.CRec 0) (Patterns.CRec 0) (@ExprCore.App typ func)) ::
-	  (Patterns.CAbs (CCall (reify_scheme typ)) (CRec 0) (@ExprCore.Abs typ func)) :: nil))).
-
-  Polymorphic Instance Reify_func' (rf : list (Command (expr typ func))) : Reify (expr typ func) := {
-    reify_scheme := reify_func' rf
+  Polymorphic Instance Reify_func_no_table (rf : list (Command (expr typ func))) : Reify (expr typ func) := {
+    reify_scheme := reify_func_no_table rf
   }.
 
 End ReifyFunc.
@@ -76,5 +74,5 @@ End ReifyFunc.
 Arguments reify_func _ _ {_ _} _.
 Arguments Reify_func _ _ {_ _} _.
 
-Arguments reify_func' _ _ {_} _.
-Arguments Reify_func' _ _ {_} _.
+Arguments reify_func_no_table _ _ {_} _.
+Arguments Reify_func_no_table _ _ {_} _.
